theories/iris/rules/iris_rules_bind.v
@@ -15,6 +15,120 @@ Section bind_rules.
 Context `{!wasmG Σ}.
 
   Lemma wp_frame_bind (s : stuckness) (E : coPset) (Φ : iris.val -> iProp Σ) n f f0 LI :
+    iris.to_val [AI_local n f LI] = None ->
+    ↪[frame] f0 -∗
+     (↪[frame] f -∗ WP LI @ s; E {{ w, ∃ f, (↪[frame] f0 -∗ WP of_val w @ s; E FRAME n; f {{ w, Φ w }}) ∗ ↪[frame] f }}) -∗
+     WP LI @ s; E FRAME n; f {{ w, Φ w }}.
+  Proof.
+    iIntros (Hetov') "Hframe H".
+    rewrite wp_frame_rewrite.
+    iLöb as "IH" forall (s E LI f f0 Hetov').
+    (* iApply wp_unfold. *)
+    destruct (iris.to_val (LI)) as [vs|] eqn:Hetov.
+    { iApply wp_unfold.
+      unfold wp_pre. simpl language.to_val. rewrite Hetov'; simpl.
+      iIntros (σ ns κ κs nt) "Hσ".
+      destruct σ as [[ ? ?] ?].
+      iDestruct "Hσ" as "(H1&H2&H3&H4&Hff&H5&H6)".
+      iDestruct (ghost_map_lookup with "Hff Hframe") as %Hlook.
+      iMod (ghost_map_update f with "Hff Hframe") as "[Hff Hframe]".
+      iDestruct ("H" with "Hframe") as "H".
+      iDestruct (wp_unfold with "H") as "H".
+      rewrite /wp_pre /= Hetov.
+      iMod ("H") as "Hf".
+      iDestruct "Hf" as (f') "[H Hf]".
+      rewrite wp_frame_rewrite.
+      iDestruct (ghost_map_lookup with "Hff Hf") as %Hlook'.
+      iMod (ghost_map_update f0 with "Hff Hf") as "[Hff Hf]".
+      rewrite !insert_insert. rewrite lookup_insert in Hlook'. inversion Hlook'.
+      iDestruct ("H" with "Hf") as "H".
+      iDestruct (wp_unfold with "H") as "H".
+      rewrite /wp_pre /=.
+      apply of_to_val in Hetov as Heq. rewrite Heq.
+      subst f. rewrite Hetov'.
+      rewrite lookup_insert in Hlook;inversion Hlook.
+      iSpecialize ("H" $! (_,_,_) 0 κ [] 0 with "[$H1 $H2 $H3 $H4 $H5 $H6 $Hff]").
+      iMod "H" as "[? H]". iModIntro. iFrame. }
+    { iApply wp_unfold. unfold wp_pre. simpl. rewrite Hetov'.
+      iIntros (σ ns κ κs nt) "Hσ".
+      destruct σ as [[ ? ?] ?].
+      iDestruct "Hσ" as "(H1&H2&H3&H4&Hff&H5&H6)".
+      iDestruct (ghost_map_lookup with "Hff Hframe") as %Hlook.
+      rewrite lookup_insert in Hlook;inversion Hlook.
+      
+      iMod (ghost_map_update f with "Hff Hframe") as "[Hff Hframe]".
+      rewrite insert_insert.
+      iDestruct ("H" with "Hframe") as "H". destruct f.
+      iDestruct (wp_unfold with "H") as "H". rewrite /wp_pre /= Hetov.
+      iSpecialize ("H" $! (_,_,_) 0 κ [] 0). 
+      iDestruct ("H" with "[$H1 $H2 $H3 $H4 $H5 $H6 $Hff]") as "H".
+
+      iMod "H" as "[%Hred H]".
+      iModIntro. iSplit.
+      { iPureIntro. destruct s =>//.
+        destruct Hred as [x [e' [σ' [efs Hstep]]]].
+        destruct σ' as [[ ? ?] ?].
+        eexists x,[AI_local n {| f_locs := l0; f_inst := i0 |} e'],(_,l,i),efs.
+        simpl. destruct Hstep as [Hstep [-> ->]]. split;auto.
+        apply r_local. eauto. }
+
+      iIntros (e2 σ2 efs Hstep).
+      destruct σ2 as [[ ? ?] ?].
+      destruct Hstep as [Hstep [-> ->]].
+      apply reduce_det_local in Hstep as Hstep';[|auto].
+      destruct Hstep' as [es2' [f1 [Heq1 [Heq2 Hstep']]]].
+      simplify_eq. destruct f1.
+      iSpecialize ("H" $! _ (_,_,_) _ with "[]").
+      { iPureIntro. split;eauto. }
+
+      repeat iMod "H". iModIntro. iNext.
+      repeat iMod "H". simpl.
+      iDestruct "H" as "[H Hf]".
+      iDestruct "Hf" as (f1) "[Hf Hcont]".
+      iDestruct "H" as "(H1&H2&H3&H4&Hff&H5&H6)".
+      iDestruct (ghost_map_lookup with "Hff Hf") as %Hlook'.
+      rewrite lookup_insert in Hlook'. inversion Hlook'.
+      iDestruct "Hcont" as "[Hcont _]".
+      subst f1.
+
+      destruct (iris.to_val [AI_local n {| f_locs := f_locs0; f_inst := f_inst0 |} es2']) eqn:Hsome.
+      { apply to_val_local_inv in Hsome as Hsome'.
+        destruct Hsome' as [tf [h [w [vh Heq]]]]. subst v.
+        apply to_val_call_host_local in Hsome as Heq.
+        destruct Heq as [LI' [Heq HLI]].
+        erewrite app_nil_l, app_nil_r in Heq. inversion Heq;subst.
+        iDestruct ("Hcont" with "Hf") as "Hcont".
+        iDestruct (wp_unfold with "Hcont") as "Hcont".
+        rewrite /wp_pre /= HLI.
+        iMod "Hcont" as "Hf".
+        iDestruct "Hf" as (f) "[Hcont Hf]".
+        iFrame.
+        iDestruct (ghost_map_lookup with "Hff Hf") as %Hlook2.
+        rewrite lookup_insert in Hlook2. inversion Hlook2. simplify_eq.
+        iMod (ghost_map_update {| f_locs := l0; f_inst := i0 |} with "Hff Hf") as "[Hff Hframe]".
+        rewrite insert_insert. iFrame.
+
+        iApply fupd_mask_intro_subseteq;[solve_ndisj|].
+        iExists _. iFrame. iSplit =>//. iIntros "Hf". iApply wp_fupd.
+        iApply wp_value;[unfold IntoVal;eapply of_to_val;eauto|].
+        iDestruct ("Hcont" with "Hf") as "Hcont".
+        iDestruct (wp_unfold with "Hcont") as "Hcont".
+        eassert (iris.to_val [AI_local n {| f_locs := f_locs0; f_inst := f_inst0 |}
+                                       (iris.of_val (callHostV tf h w (No_local vh)))]
+                = Some (callHostV tf h w (One_local [] n {| f_locs := f_locs0; f_inst := f_inst0 |} vh []))) as Hetov2.
+        { erewrite of_to_val;[|eauto].
+          apply to_val_local_add_frame. auto. }
+        rewrite /wp_pre /= Hetov2. iFrame. }
+      
+      iMod (ghost_map_update {| f_locs := l0; f_inst := i0 |} with "Hff Hf") as "[Hff Hframe]".
+      rewrite insert_insert.
+      simpl. iApply fupd_mask_intro_subseteq;[solve_ndisj|]. iFrame.
+      iExists _. iFrame. iSplit =>//. iIntros "Hf".
+      iApply ("IH" with "[] Hf Hcont");[auto|..].
+    }
+  Qed.
+
+  Lemma wp_frame_bind (s : stuckness) (E : coPset) (Φ : iris.val -> iProp Σ) n f f0 LI :
     ↪[frame] f0 -∗
      (↪[frame] f -∗ WP LI @ s; E {{ w, ∃ f, (↪[frame] f0 -∗ WP of_val w @ s; E FRAME n; f {{ w, Φ w }}) ∗ ↪[frame] f }}) -∗
      WP LI @ s; E FRAME n; f {{ w, Φ w }}.
